\documentclass{memoir}
\usepackage{amsmath}
\usepackage{amsthm}
\usepackage{amssymb}
\usepackage{commath}
\theoremstyle{plain}
\newtheorem{theorem}{Theorem}

\theoremstyle{definition}
\newtheorem{example}{Example}

\begin{document}
Let $v_\infty \in V$.
Fix a planar embedding of $G=(V,E)$ and $G^* = (V^*, E^*)$.

\begin{theorem}
Consider variables $x_e$ for all $e\in E$. 
Consider also variables $z_{e,v}$ for all $e\in E\setminus\delta(v_\infty)$
and $v\in V^*$ with $v\in e^*$.

The following with the projection map to $x$-variables is an extended formulation of SEP.

\begin{align}
x_e + z_{e,v}+z_{e,u} &= 1 & v_\infty \not\in e \in E, e^* = \cbr{u,v} \in V^* \label{oneuse} \\
\sum_{e\in\delta(v)} z_{e,v} &= 1 & v\in V^*, \text{$v$ is not incident to $v$} \label{facedegree} \\
x(\delta(v)) &= 2 & v\in V \label{vertexdegree} \\
(x,z) &\geq 0
\end{align}
\end{theorem}


\begin{theorem}
For $S\subseteq E$, define

$$z(S) = \sum_{\substack{v_\infty\not\in e\in S \\ e^* = \cbr{u,v}}} z_{e,u} + z_{e,v}$$

For $S\subseteq V$, define 

$$z(\partial^-(S)) = \sum_{\substack{e \in \gamma(S) \\ e^* = \cbr{u,v} \\ \text{$v$ is in a face of $G[S]$ that contains $v_\infty$ in its interior}}} z_{e,v}$$


Let $(H, T_1, \cdots, T_k)$ be a comb with the property that for any $S\in\cbr{H, T_1,\cdots, T_k}$, $G[S]$ and $G[V\setminus S]$ are both connected. If any of these sets $S$ contains $v_\infty$,
replace it with $V\setminus S$.
The following is a Chv\'{a}tal cut on the extended formulation of SEP.

$$z(\partial^-(H)) +  \sum_{i=1}^k z(\partial^-(T_i)) \geq \frac{k-1}{2}$$



\end{theorem}

\begin{proof}
Let $S$ be any of $H, T_1,\cdots, T_k$. Note that $v_\infty\not\in S$.

\begin{align*}
&\phantom{{}={}} x(\delta(S)) - 2z(\gamma(S)) \\ 
&= \del{\sum_{v\in S} x(\delta(v)) - 2x(\gamma(S))} - 2z(\gamma(S))\\
&= 2\abs{S} - 2x(\gamma(S)) - 2z(\gamma(S)) \tag*{by \eqref{vertexdegree}} \\
&= 2\abs{S} - 2\del{x(\gamma(S)) + z(\gamma(S))} \\
&= 2\abs{S} - 2\del{\sum_{e = \cbr{u,v}\in \gamma(S)} x_e + z_{e,u} + z_{e,v} } \\
&= 2\abs{S} - 2\abs{\gamma(S)} \tag*{by \eqref{oneuse} since $v_\infty\not\in S$ and hence $\delta(v_\infty)\cap \gamma(S) = \varnothing$} \\
&= 2\del{\abs{S}-\abs{\gamma(S)}} \\
&= 2\del{2 - \abs{F(G[S])}} \tag*{by Euler's formula} \\ 
z(\gamma(S)) &= \frac{1}{2}x(\delta(S)) - 2 + \abs{F(G[S])} \\
z(\gamma(S)) - \abs{F(G[S])} &= \frac{1}{2}x(\delta(S)) - 2
\end{align*}

Now, since $G[S]$ and $G[V\setminus S]$ are connected, at most one face $f$ of $F(G[S])$ is not a face of $G$. Since $v_\infty\not\in S$, $v_\infty$ is contained in the interior of $f$.

Note that
\begin{align*}
z(\gamma(S)) - \abs{F(G[S])} &= z(\gamma(S)) - \sum_{v \in F(G[S])} 1 \\
&= z(\gamma(S)) - 1 - \sum_{\substack{v \in F(G[S]) \\ v\neq f}} \sum_{e\in\delta(v)} z_{e,v} \tag*{by \eqref{facedegree}} \\
&= z(\partial^-(S)) - 1 \\
z(\partial^-(S)) &= \frac{1}{2}x(\delta(S)) - 1
\end{align*}

Summing over handles and teeth and applying the comb inequality:

\begin{align*}
z(\partial^-(H)) + \sum_{i=1}^k z(\partial^-(T_i)) &\geq \frac{1}{2}(3k+1) - (k+1) \\
&= \frac{k-1}{2}
\end{align*}
\end{proof}

\begin{example}
	Consider $\texttt{bowtieGraph.py}$ with $v_\infty = p_6$. 
	It has noninteger optimum $\del{x_1=x_2=x_4=x_7=x_8=x_9=z_{1,1}=z_{2,2}=z_{4,1}=z_{7,2} = \frac{1}{2}, x_4=x_5=x_6 = 1}$.
	Let

	\begin{align*}
		H &= \cbr{p_1, p_2, p_3} \\
		T_1 &= \cbr{p_1, p_5} \\
		T_2 &= \cbr{p_3, p_4} \\
		T_3 &= \cbr{p_2, p_6}
	\end{align*}

	Then $\del{H,T_1,T_2,T_3}$ is a comb. Since $v_\infty = p_6 \in T_3$, we replace
	$T_3$ with $V\setminus T_3$. Then the following is a cutting plane:

	\begin{verbatim}
	z1,5+z2,2+z4,3+z3,2+z3,5+z6,2+z6,3+z2,1+z3,5+z6,3+z7,4 >= 1
	\end{verbatim}

	Accordingly,

	\begin{align*}
		&\phantom{{}={}} \del{z_{1,5}+z_{2,2}+z_{4,3}}+\del{z_{3,2}+z_{3,5}}+\del{z_{6,2}+z_{6,3}}+\del{z_{2,1}+z_{3,5}+z_{6,3}+z_{7,4}} \\ 
		&= z(\delta^-(H)) + z(\delta^-(T_1)) + z(\delta^-(T_2)) + z(\delta^-(V\setminus T_3)) \\
		&\geq 1
	\end{align*}

\end{example}

\end{document}
